Linked list example

pulse/examples/steel/arraystructs/ListNode.fst
@@ -8,44 +8,39 @@ open Steel.Effect
 open FStar.PCM
 open FStar.PCM.POD
 open Steel.C.PCM
+module U = FStar.Universe
 
 type node_field = | Value | Next
 
-let ref' a b = pb: Ghost.erased (pcm b) & ref a pb
-
-//let node_fields node k = match k with
-//  | Value -> pod (FStar.Universe.raise_t int)
-//  | Next -> pod (option (ref' (FStar.Universe.raise_t node) node))
-
-let node_fields (node:Type) k = match k with
-  | Value -> pod (Universe.raise_t int)
+let node_fields (node:Type u#1) k : Type u#1 = match k with
+  | Value -> pod int'
   | Next -> pod (option (ref' node node))
 
 #push-options "--__no_positivity"
-noeq type node =
+noeq type node: Type u#1 =
 { un_node: restricted_t node_field (node_fields node) }
 #pop-options
 
+let node': Type u#1 = restricted_t node_field (node_fields node)
+
 let node_fields_pcm k: pcm (node_fields node k) = match k with
-  | Value -> pod_pcm (FStar.Universe.raise_t int)
+  | Value -> pod_pcm int'
   | Next -> pod_pcm (option (ref' node node))
 
-let node_pcm' = prod_pcm node_fields_pcm
+let node_pcm': pcm node' = prod_pcm node_fields_pcm
 
-let node_pcm: pcm node =
-  let p: FStar.PCM.pcm node = {
-    FStar.PCM.p = {
-      composable = (fun x y -> composable node_pcm' x.un_node y.un_node);
-      op = (fun x y -> Mknode (op node_pcm' x.un_node y.un_node));
-      one = Mknode (one node_pcm');
-    };
-    comm = (fun x y -> node_pcm'.comm x.un_node y.un_node);
-    assoc = (fun x y z -> node_pcm'.assoc x.un_node y.un_node z.un_node);
-    assoc_r = (fun x y z -> node_pcm'.assoc_r x.un_node y.un_node z.un_node);
-    is_unit = (fun x -> node_pcm'.is_unit x.un_node);
-    refine = (fun x -> node_pcm'.refine x.un_node);
-  } in
-  p
+let node_pcm: pcm node = {
+  FStar.PCM.p = {
+    composable = (fun x y -> composable node_pcm' x.un_node y.un_node);
+    op = (fun x y -> Mknode (op node_pcm' x.un_node y.un_node));
+    one = Mknode (one node_pcm');
+  };
+  comm = (fun x y -> node_pcm'.comm x.un_node y.un_node);
+  assoc = (fun x y z -> node_pcm'.assoc x.un_node y.un_node z.un_node);
+  assoc_r = (fun x y z -> node_pcm'.assoc_r x.un_node y.un_node z.un_node);
+  is_unit = (fun x -> node_pcm'.is_unit x.un_node);
+  refine = (fun x -> node_pcm'.refine x.un_node);
+}
 
 let roll: node_pcm' `morphism` node_pcm = {
   morph = Mknode;
@@ -67,21 +62,7 @@ let roll_compatible x v
     (requires compatible node_pcm' x v)
     (ensures compatible node_pcm (Mknode x) (Mknode v))
     [SMTPat (compatible node_pcm' x v)]
-= let frame = compatible_elim node_pcm' x v in
-  compatible_intro node_pcm (Mknode x) (Mknode v) (Mknode frame)
-
-val compatible_morphism
-  (#p: pcm 'a) (#q: pcm 'b)
-  (f: p `morphism` q)
-  (x y: Ghost.erased 'a)
-: Lemma
-    (requires compatible p x y)
-    (ensures compatible q (f.morph x) (f.morph y))
-
-let compatible_morphism #a #b #p #q f x y =
-  let frame_x = compatible_elim p x y in
-  let _ = f.morph_compose frame_x x in
-  compatible_intro q (f.morph x) (f.morph y) (f.morph frame_x)
+= compatible_morphism roll x v
 
 let unroll_compatible x v
 : Lemma
@@ -136,115 +117,140 @@ let unroll_conn: node_pcm `connection` node_pcm' = {
   conn_lift_frame_preserving_upd = unroll_conn_lift_fpu;
 }
 
-let mk_node' (value: Ghost.erased _) (next: Ghost.erased _): Ghost.erased _ =
-  Ghost.hide (fun k -> match k with
+let mk_node'_f (value: pod int') (next: pod (option (ref' node node)))
+  (k: node_field)
+: node_fields node k
+= match k with
   | Value -> value
-  | Next -> next)
+  | Next -> next
+  
+let mk_node'
+  (value: Ghost.erased (pod int'))
+  (next: Ghost.erased (pod (option (ref' node node))))
+: Ghost.erased node'
+= Ghost.hide (on_domain node_field (mk_node'_f (Ghost.reveal value) (Ghost.reveal next)))
 
-let mk_node (value: Ghost.erased _) (next: Ghost.erased _): Ghost.erased _ =
-  Ghost.hide (mk_node' (Ghost.reveal value) (Ghost.reveal next))
+let mk_node value next = Ghost.hide (Mknode (mk_node' (Ghost.reveal value) (Ghost.reveal next)))
 
 let _value
-: node_pcm `connection` pod_pcm (FStar.Universe.raise_t int)
+: node_pcm `connection` pod_pcm int'
 = unroll_conn `connection_compose` struct_field node_fields_pcm Value
 
 let _next
 : node_pcm `connection` pod_pcm (option (ref' node node))
 = unroll_conn `connection_compose` struct_field node_fields_pcm Next
 
-let one_next : Ghost.erased (pod (Universe.raise_t int)) =
-  Ghost.hide (one (pod_pcm (FStar.Universe.raise_t int)))
+let one_next : Ghost.erased (pod int') =
+  Ghost.hide (one (pod_pcm int'))
 
-let addr_of_next
-  (#value:Ghost.erased (pod (Universe.raise_t int)))
+let node'_without_value value next
+: Lemma (struct_without_field node_fields_pcm Value (mk_node' value next) `feq`
+         Ghost.reveal (mk_node' none next))
+  [SMTPat (mk_node' value next)]
+= ()
+
+let node'_with_value value next
+: Lemma (struct_with_field node_fields_pcm Value (Ghost.reveal value) (mk_node' none next) `feq`
+         Ghost.reveal (mk_node' value next))
+  [SMTPat (mk_node' value next)]
+= ()
+
+let node'_without_next value next
+: Lemma (struct_without_field node_fields_pcm Next (mk_node' value next) `feq`
+         Ghost.reveal (mk_node' value none))
+  [SMTPat (mk_node' value next)]
+= ()
+
+let node'_with_next value next
+: Lemma (struct_with_field node_fields_pcm Next (Ghost.reveal next) (mk_node' value none) `feq`
+         Ghost.reveal (mk_node' value next))
+  [SMTPat (mk_node' value next)]
+= ()
+
+let mk_node_mk_node' value next
+: Lemma (
+    Ghost.reveal (mk_node value next) ==
+    unroll_conn.conn_small_to_large.morph (mk_node' value next))
+= ()
+
+let unroll_ref 
+  (#value:Ghost.erased (pod int'))
   (#next:Ghost.erased (pod (option (ref' node node))))
   (p: ref 'a node_pcm)
-: SteelT (q:ref 'a (pod_pcm (FStar.Universe.raise_t int)){q == ref_focus p _value})
+: SteelT (p':ref 'a node_pcm'{p' == ref_focus p unroll_conn})
+    (p `pts_to` mk_node value next)
+    (fun p' -> p' `pts_to` mk_node' value next)
+= let p' = focus p unroll_conn (mk_node value next) (mk_node' value next) in
+  A.return p'
+
+let roll_ref 
+  (#value:Ghost.erased (pod int'))
+  (#next:Ghost.erased (pod (option (ref' node node))))
+  (p: ref 'a node_pcm) (p': ref 'a node_pcm')
+: Steel unit
+    (p' `pts_to` mk_node' value next)
+    (fun _ -> p `pts_to` mk_node value next)
+    (requires fun _ -> p' == ref_focus p unroll_conn)
+    (ensures fun _ _ _ -> True)
+= unfocus p' p unroll_conn (mk_node' value next);
+  A.change_equal_slprop (p `pts_to` _) (p `pts_to` _)
+
+let addr_of_value
+  (#value:Ghost.erased (pod int'))
+  (#next:Ghost.erased (pod (option (ref' node node))))
+  (p: ref 'a node_pcm)
+: SteelT (q:ref 'a (pod_pcm int'){q == ref_focus p _value})
     (p `pts_to` mk_node value next)
     (fun q ->
-       (p `pts_to` mk_node one_next next) `star`
+       (p `pts_to` mk_node none next) `star`
        (q `pts_to` value))
-= A.sladmit(); A.return (admit())
+= let p' = unroll_ref p in
+  let q = addr_of_struct_field p' Value (mk_node' value next) in
+  A.change_equal_slprop (p' `pts_to` _) (p' `pts_to` mk_node' none next);
+  A.change_equal_slprop (q `pts_to` _) (q `pts_to` value);
+  roll_ref p p';
+  A.return q
 
-//let node_pcm: pcm (restricted_t 
-//node --> prod_pcm node_pcm_fields
+let unaddr_of_value
+  (#value:Ghost.erased (pod int'))
+  (#next:Ghost.erased (pod (option (ref' node node))))
+  (p: ref 'a node_pcm)
+  (q: ref 'a (pod_pcm int'){q == ref_focus p _value})
+: SteelT unit
+    ((p `pts_to` mk_node none next) `star` (q `pts_to` value))
+    (fun _ -> p `pts_to` mk_node value next)
+= let p' = unroll_ref p in
+  let q = unaddr_of_struct_field Value q p' (mk_node' none next) value in
+  A.change_equal_slprop (p' `pts_to` _) (p' `pts_to` mk_node' value next);
+  roll_ref p p';
+  A.return ()
 
-// #push-options "--print_universes"
-// 
-// let x = 3
-// 
-// #pop-options
-// 
-// type node = {
-// }
-// 
-// let node_fields k: Type = match k with
-//   | I -> pod int
-//   | Next -> uninit_t (pod rec_arg)
-//   
-// let node (rec_arg:Type): Type = restricted_t node_field (node_fields rec_arg)
-// 
-// /// PCM for node:
-// 
-// let node_fields_pcm k : pcm (node_fields k) = match k with
-//   | P1 -> point_pcm
-//   | P2 -> point_pcm
-// let node_pcm = prod_pcm node_fields_pcm
-// 
-// /// (mk_node p1 p2) represents (struct node){.p1 = p1, .p2 = p2}
-// 
-// let mk_node_f (p1 p2: point) (k: node_field): node_fields k = match k with
-//   | P1 -> p1
-//   | P2 -> p2
-// let mk_node p1 p2 = on_domain node_field (mk_node_f (Ghost.reveal p1) (Ghost.reveal p2))
-// 
-// let _p1 = struct_field node_fields_pcm P1
-// let _p2 = struct_field node_fields_pcm P2
-// 
-// /// Taking pointers to the p1 and p2 fields of a node
-// 
-// let node_without_p1 p1 p2
-// : Lemma (struct_without_field node_fields_pcm P1 (mk_node p1 p2) `feq`
-//          Ghost.reveal (mk_node (one point_pcm) p2))
-//   [SMTPat (mk_node p1 p2)]
-// = ()
-// 
-// let node_with_p1 p1 p2
-// : Lemma (struct_with_field node_fields_pcm P1 (Ghost.reveal p1) (mk_node (one point_pcm) p2) `feq`
-//          Ghost.reveal (mk_node p1 p2))
-//   [SMTPat (mk_node p1 p2)]
-// = ()
-// 
-// let node_without_p2 p1 p2
-// : Lemma (struct_without_field node_fields_pcm P2 (mk_node p1 p2) `feq`
-//          Ghost.reveal (mk_node p1 (one point_pcm)))
-//   [SMTPat (mk_node p1 p2)]
-// = ()
-// 
-// let node_with_p2 p1 p2
-// : Lemma (struct_with_field node_fields_pcm P2 (Ghost.reveal p2) (mk_node p1 (one point_pcm)) `feq`
-//          Ghost.reveal (mk_node p1 p2))
-//   [SMTPat (mk_node p1 p2)]
-// = ()
-// 
-// let addr_of_p1 #a #p1 #p2 p =
-//   let q = addr_of_struct_field p P1 (mk_node p1 p2) in
-//   A.change_equal_slprop (p `pts_to` _) (p `pts_to` mk_node (one point_pcm) p2);
-//   A.change_equal_slprop (q `pts_to` _) (q `pts_to` p1);
-//   A.return q
-// 
-// let unaddr_of_p1 #a #p1 #p2 p q =
-//   unaddr_of_struct_field P1 q p (mk_node (one point_pcm) p2) p1;
-//   A.change_equal_slprop (p `pts_to` _) (p `pts_to` _)
-// 
-// let addr_of_p2 #a #p1 #p2 p =
-//   let q = addr_of_struct_field p P2 (mk_node p1 p2) in
-//   A.change_equal_slprop (p `pts_to` _) (p `pts_to` mk_node p1 (one point_pcm));
-//   A.change_equal_slprop (q `pts_to` _) (q `pts_to` p2);
-//   A.return q
-// 
-// let unaddr_of_p2 #a #p1 #p2 p q =
-//   unaddr_of_struct_field P2 q p (mk_node p1 (one point_pcm)) p2;
-//   A.change_equal_slprop (p `pts_to` _) (p `pts_to` _)
+let addr_of_next
+  (#value:Ghost.erased (pod int'))
+  (#next:Ghost.erased (pod (option (ref' node node))))
+  (p: ref 'a node_pcm)
+: SteelT (q:ref 'a (pod_pcm (option (ref' node node))){q == ref_focus p _next})
+    (p `pts_to` mk_node value next)
+    (fun q ->
+       (p `pts_to` mk_node value none) `star`
+       (q `pts_to` next))
+= let p' = unroll_ref p in
+  let q = addr_of_struct_field p' Next (mk_node' value next) in
+  A.change_equal_slprop (p' `pts_to` _) (p' `pts_to` mk_node' value none);
+  A.change_equal_slprop (q `pts_to` _) (q `pts_to` next);
+  roll_ref p p';
+  A.return q
 
-#pop-options
+let unaddr_of_next
+  (#value:Ghost.erased (pod int'))
+  (#next:Ghost.erased (pod (option (ref' node node))))
+  (p: ref 'a node_pcm)
+  (q: ref 'a (pod_pcm (option (ref' node node))){q == ref_focus p _next})
+: SteelT unit
+    ((p `pts_to` mk_node value none) `star` (q `pts_to` next))
+    (fun q -> p `pts_to` mk_node value next)
+= let p' = unroll_ref p in
+  let q = unaddr_of_struct_field Next q p' (mk_node' value none) next in
+  A.change_equal_slprop (p' `pts_to` _) (p' `pts_to` mk_node' value next);
+  roll_ref p p';
+  A.return ()
