pulse/examples/steel/arraystructs/ListNode.fsti
@@ -1,0 +1,73 @@
+module ListNode
+
+open FStar.PCM.POD
+open FStar.PCM
+open Steel.Effect
+open PointStruct
+open Steel.C.PCM
+module U = FStar.Universe
+
+let ref'_f a b (pb: Ghost.erased (pcm b)) = ref a (Ghost.reveal pb)
+let ref' a b = dtuple2 (Ghost.erased (pcm b)) (ref'_f a b)
+
+let int': Type u#1 = U.raise_t int
+
+/// struct node { int value; struct node *next; };
+
+val node: Type u#1
+
+/// PCM for node:
+
+val node_pcm: pcm node
+
+/// (mk_node value next) represents (struct node){.value = value, .next = next}
+
+val mk_node
+  (i: Ghost.erased (pod int'))
+  (next: Ghost.erased (pod (option (ref' node node))))
+: Ghost.erased node
+
+/// Lenses for fields
+
+val _value: node_pcm `connection` pod_pcm int'
+val _next: node_pcm `connection` pod_pcm (option (ref' node node))
+
+/// Taking pointers to the fields of a node
+
+val addr_of_value
+  (#value:Ghost.erased (pod int'))
+  (#next:Ghost.erased (pod (option (ref' node node))))
+  (p: ref 'a node_pcm)
+: SteelT (q:ref 'a (pod_pcm int'){q == ref_focus p _value})
+    (p `pts_to` mk_node value next)
+    (fun q ->
+       (p `pts_to` mk_node none next) `star`
+       (q `pts_to` value))
+
+val unaddr_of_value
+  (#value:Ghost.erased (pod int'))
+  (#next:Ghost.erased (pod (option (ref' node node))))
+  (p: ref 'a node_pcm)
+  (q: ref 'a (pod_pcm int'){q == ref_focus p _value})
+: SteelT unit
+    ((p `pts_to` mk_node none next) `star` (q `pts_to` value))
+    (fun q -> p `pts_to` mk_node value next)
+
+val addr_of_next
+  (#value:Ghost.erased (pod int'))
+  (#next:Ghost.erased (pod (option (ref' node node))))
+  (p: ref 'a node_pcm)
+: SteelT (q:ref 'a (pod_pcm (option (ref' node node))){q == ref_focus p _next})
+    (p `pts_to` mk_node value next)
+    (fun q ->
+       (p `pts_to` mk_node value none) `star`
+       (q `pts_to` next))
+
+val unaddr_of_next
+  (#value:Ghost.erased (pod int'))
+  (#next:Ghost.erased (pod (option (ref' node node))))
+  (p: ref 'a node_pcm)
+  (q: ref 'a (pod_pcm (option (ref' node node))){q == ref_focus p _next})
+: SteelT unit
+    ((p `pts_to` mk_node value none) `star` (q `pts_to` next))
+    (fun q -> p `pts_to` mk_node value next)
